Source/DafnyLS/Workspace/DocumentModifier.cs
@@ -8,37 +8,92 @@ using System;
 
 namespace Microsoft.Dafny.LanguageServer.Workspace{
     public class DocumentModifier{
-        private void ModifyProgram(Dafny.Program program){
-            Console.WriteLine("*************** Print Program Info ****************");
-            Console.WriteLine("Program name: " + program.FullName);
 
+        // private BlockStmt ClonedStmt;
+        // private Cloner cloner = new Cloner();
+        // private string _moduleName;
+        // private string _callableName;
+        /*
+        public DocumentModifier(Dafny.Program program, string ModuleName, string CallableName){
+            _moduleName = ModuleName;
+            _callableName = CallableName;
+            foreach(ModuleDefinition module in program.ModuleSigs.Keys){
+                if(module.FullName != _moduleName) continue;
+                foreach(ICallable callable in module.CallGraph.vertices.Keys){
+                    if(callable.NameRelativeToModule != _callableName) continue;
+                    var LemmaCallable = (Lemma)callable;
+                    var Body = LemmaCallable.methodBody;
+                    // Console.WriteLine("********** Print Original Statement Info ************");
+                    // Console.WriteLine("Cloned Statement count: " + Body.Body.Count);
+                    for(int i = 0; i < Body.Body.Count; ++ i){
+                        DocumentPrinter.PrintStatementInfo(Body.Body[i], "Test ", i, 0);
+                    }
+                    ClonedStmt = cloner.CloneBlockStmt(Body);
+                    // Console.WriteLine("********** Print Cloned Statement Info ************");
+                    // Console.WriteLine("Cloned Statement count: " + ClonedStmt.Body.Count);
+                    for(int i = 0; i < ClonedStmt.Body.Count; ++ i){
+                        DocumentPrinter.PrintStatementInfo(ClonedStmt.Body[i], "Test ", i, 0);
+                    }
+                    break;
+                }
+            }
+        }*/
+        /*
+        public void RestoreProgram(Dafny.Program program){
+            foreach(ModuleDefinition module in program.ModuleSigs.Keys){
+                if(module.FullName != _moduleName) continue;
+                foreach(ICallable callable in module.CallGraph.vertices.Keys){
+                    if(callable.NameRelativeToModule != _callableName) continue;
+                    var LemmaCallable = (Lemma)callable;
+                    LemmaCallable.methodBody = cloner.CloneBlockStmt(ClonedStmt);
+                }
+            }
+        }*/
+
+        public static void RemoveLastLineOfFOO(Dafny.Program program){
             Console.WriteLine("Program module signature size: " + program.ModuleSigs.Count);
             int module_count = 0;
             foreach(ModuleDefinition module in program.ModuleSigs.Keys){
                 Console.WriteLine("   Module "+module_count+" full name: " + module.FullName);
-                Console.WriteLine("   Module "+module_count+" include size: " + module.Includes.Count);
-                Console.WriteLine("   Module "+module_count+" TopLevelDecls size: " + module.TopLevelDecls.Count);
-
-                Console.WriteLine("   Module "+module_count+" call graph size: " + module.CallGraph.vertices.Count);
                 int callable_count = 0;
                 foreach(ICallable callable in module.CallGraph.vertices.Keys){
-                var corresVertex = module.CallGraph.vertices[callable];
-                Console.WriteLine("     Callable "+callable_count+" kind: " + callable.WhatKind);
-                Console.WriteLine("     Callable "+callable_count+" name: " + callable.NameRelativeToModule);
-                Console.WriteLine("     Callable "+callable_count+" #succesor: " + corresVertex.Successors.Count);
-                if(callable.WhatKind == "lemma"){
-                    var MethodCallable = (Method)callable;
-                    var Body = MethodCallable.methodBody;
-                    Console.WriteLine("     Callable "+callable_count+" #statement " + Body.Body.Count);
-                    // Try to remove the last assertion of foo
-                    if(callable.NameRelativeToModule == "foo"){
-                    Body.Body.Remove(Body.Body.Last());
-                    Console.WriteLine("     Callable "+callable_count+" #statement after deletion " + Body.Body.Count);
+                    var corresVertex = module.CallGraph.vertices[callable];
+                    Console.WriteLine("     Callable "+callable_count+" name: " + callable.NameRelativeToModule);
+                    if(callable.WhatKind == "lemma"){
+                        var LemmaCallable = (Lemma)callable;
+                        var Body = LemmaCallable.methodBody;
+                        Console.WriteLine("     Callable "+callable_count+" #statement " + Body.Body.Count);
+                        // Try to remove the last assertion of foo
+                        if(callable.NameRelativeToModule == "foo"){
+                            Body.Body.Remove(Body.Body.Last());
+                            Console.WriteLine("     Callable "+callable_count+" #statement after deletion " + Body.Body.Count);
+                        }
                     }
-                }
-                ++ callable_count;
+                    ++ callable_count;
                 }
                 ++module_count;
+            }
+        }
+        public static void RemoveLemmaLines(Dafny.Program program, string LemmaName, string ModuleName, int Start){
+            // Console.WriteLine("Program module signature size: " + program.ModuleSigs.Count);
+            foreach(ModuleDefinition module in program.ModuleSigs.Keys){
+                if(module.FullName != ModuleName) continue;
+                //Console.WriteLine("   Module "+module_count+" full name: " + module.FullName);
+                foreach(ICallable callable in module.CallGraph.vertices.Keys){
+                    var corresVertex = module.CallGraph.vertices[callable];
+                    // Console.WriteLine("     Callable "+callable_count+" name: " + callable.NameRelativeToModule);
+                    if(callable.WhatKind != "lemma") continue;
+                    if(callable.NameRelativeToModule != LemmaName) continue;
+                    var LemmaCallable = (Lemma)callable;
+                    var Body = LemmaCallable.methodBody;
+                    // Console.WriteLine("     Callable "+callable_count+" #statement " + Body.Body.Count);
+                    /*
+                    if(Start >= Body.Body.Count){
+                        Console.WriteLine("Cannot starting position longer than list size!");
+                        return;
+                    }*/
+                    Body.Body.RemoveRange(Start, Body.Body.Count - Start);
+                }
             }
         }
     }
