Source/DafnyLS/Workspace/TextDocumentLoader.cs
@@ -29,6 +29,7 @@ namespace Microsoft.Dafny.LanguageServer.Workspace {
     }
 
     public async Task<DafnyDocument> LoadAsync(TextDocumentItem textDocument, bool verify, CancellationToken cancellationToken) {
+      /*
       Console.WriteLine("************** Start loading the target file asynchronously!!! **************");
       var errorReporter = new BuildErrorReporter();
       var program = await _parser.ParseAsync(textDocument, errorReporter, cancellationToken);
@@ -36,13 +37,22 @@ namespace Microsoft.Dafny.LanguageServer.Workspace {
       var compilationUnit = await _symbolResolver.ResolveSymbolsAsync(textDocument, program, cancellationToken);
       // DocumentPrinter.OutputProgramInfo(program);
       var symbolTable = _symbolTableFactory.CreateFrom(program, compilationUnit, cancellationToken);
-      DocumentPrinter.OutputProgramInfo(program);
+      // DocumentPrinter.OutputProgramInfo(program);
+      // DocumentModifier.RemoveLastLineOfFOO(program);
+      
       var serializedCounterExamples = await VerifyIfEnabled(textDocument, program, verify, cancellationToken);
       // DocumentPrinter.OutputProgramInfo(program);
-      DocumentPrinter.OutputErrorInfo(errorReporter);
-      return new DafnyDocument(textDocument, errorReporter, program, symbolTable, serializedCounterExamples);
+      // DocumentPrinter.OutputErrorInfo(errorReporter);
+      // var serializedCounterExamples = await VerifyTwiceWithModificationFirst(textDocument, program, verify, cancellationToken);
+      return new DafnyDocument(textDocument, errorReporter, program, symbolTable, serializedCounterExamples);*/
+      if(verify){
+        return await GenerateProgramAssertionTestBasic(textDocument ,cancellationToken);
+      }
+      else{
+        return await GenerateProgramWithoutVerify(textDocument, cancellationToken);
+      }
     }
-
+    /*
     private async Task<string?> VerifyIfEnabled(TextDocumentItem textDocument, Dafny.Program program, bool verify, CancellationToken cancellationToken) {
       if(!verify) {
         Console.WriteLine("*************** Not verifying this time ****************");
@@ -54,6 +64,129 @@ namespace Microsoft.Dafny.LanguageServer.Workspace {
       _notificationPublisher.Completed(textDocument, serializedCounterExamples == null);
       Console.WriteLine("*************** Verify Complete ****************");
       return serializedCounterExamples;
+    }*/
+
+    private async Task<DafnyDocument> GenerateProgramWithSmallTweak(TextDocumentItem textDocument, CancellationToken cancellationToken){
+      var errorReporter = new BuildErrorReporter();
+      var program = await _parser.ParseAsync(textDocument, errorReporter, cancellationToken);
+      var compilationUnit = await _symbolResolver.ResolveSymbolsAsync(textDocument, program, cancellationToken);
+      var symbolTable = _symbolTableFactory.CreateFrom(program, compilationUnit, cancellationToken);
+      // Verify 
+      _notificationPublisher.Started(textDocument);
+      DocumentModifier.RemoveLemmaLines(program, "foo", "module1", 3);
+      var serializedCounterExamples = await _verifier.VerifyAsync(program, cancellationToken);
+      DocumentPrinter.OutputProgramInfo(program);
+      DocumentPrinter.OutputErrorInfo(errorReporter);
+
+      errorReporter = new BuildErrorReporter();
+      program = await _parser.ParseAsync(textDocument, errorReporter, cancellationToken);
+      compilationUnit = await _symbolResolver.ResolveSymbolsAsync(textDocument, program, cancellationToken);
+      symbolTable = _symbolTableFactory.CreateFrom(program, compilationUnit, cancellationToken);
+      serializedCounterExamples = await _verifier.VerifyAsync(program, cancellationToken);
+      _notificationPublisher.Completed(textDocument, serializedCounterExamples == null);
+      DocumentPrinter.OutputProgramInfo(program);
+      DocumentPrinter.OutputErrorInfo(errorReporter);
+
+      return new DafnyDocument(textDocument, errorReporter, program, symbolTable, serializedCounterExamples);
+    }
+
+    private async Task<DafnyDocument> GenerateProgram(TextDocumentItem textDocument, CancellationToken cancellationToken){
+      var errorReporter = new BuildErrorReporter();
+      var program = await _parser.ParseAsync(textDocument, errorReporter, cancellationToken);
+      var compilationUnit = await _symbolResolver.ResolveSymbolsAsync(textDocument, program, cancellationToken);
+      var symbolTable = _symbolTableFactory.CreateFrom(program, compilationUnit, cancellationToken);
+      _notificationPublisher.Started(textDocument);
+      var serializedCounterExamples = await _verifier.VerifyAsync(program, cancellationToken);
+      // DocumentPrinter.OutputErrorInfo(errorReporter);
+      _notificationPublisher.Completed(textDocument, serializedCounterExamples == null);
+      // DocumentPrinter.OutputErrorInfo(errorReporter);
+      return new DafnyDocument(textDocument, errorReporter, program, symbolTable, serializedCounterExamples);
+    }
+
+    private async Task<DafnyDocument> GenerateProgramWithoutVerify(TextDocumentItem textDocument, CancellationToken cancellationToken){
+      var errorReporter = new BuildErrorReporter();
+      var program = await _parser.ParseAsync(textDocument, errorReporter, cancellationToken);
+      var compilationUnit = await _symbolResolver.ResolveSymbolsAsync(textDocument, program, cancellationToken);
+      var symbolTable = _symbolTableFactory.CreateFrom(program, compilationUnit, cancellationToken);
+      return new DafnyDocument(textDocument, errorReporter, program, symbolTable, null);
+    }
+
+    private async Task<DafnyDocument> GenerateProgramAssertionTestBasic(TextDocumentItem textDocument, CancellationToken cancellationToken){
+      int begin = 0;    // Beginning of the target search range
+      int end = 0;      // End of the target search range
+      string ModuleName = "module1";
+      string LemmaName = "foo";
+      
+      _notificationPublisher.Started(textDocument);
+
+      // Initial run, to record program info
+      var errorReporter = new BuildErrorReporter();
+      var program = await _parser.ParseAsync(textDocument, errorReporter, cancellationToken);
+      var compilationUnit = await _symbolResolver.ResolveSymbolsAsync(textDocument, program, cancellationToken);
+      var symbolTable = _symbolTableFactory.CreateFrom(program, compilationUnit, cancellationToken);
+      // Record the program info
+      foreach(ModuleDefinition module in program.ModuleSigs.Keys){
+          if(module.FullName != ModuleName) continue;
+          foreach(ICallable callable in module.CallGraph.vertices.Keys){
+              var corresVertex = module.CallGraph.vertices[callable];
+              if(callable.WhatKind != "lemma" || callable.NameRelativeToModule != LemmaName) continue;
+              var LemmaCallable = (Lemma)callable;
+              end = LemmaCallable.methodBody.Body.Count;
+          }
+      }
+      var serializedCounterExamples = await _verifier.VerifyAsync(program, cancellationToken);
+      if(errorReporter.AllMessages[ErrorLevel.Error].Count == 0){
+        _notificationPublisher.Completed(textDocument, serializedCounterExamples == null);
+        return new DafnyDocument(textDocument, errorReporter, program, symbolTable, serializedCounterExamples);
+      }
+      if(errorReporter.AllMessages[ErrorLevel.Error].Count != 0 && end == 0){
+        Console.WriteLine("The error is not in the designated lemma or module");
+        _notificationPublisher.Completed(textDocument, serializedCounterExamples == null);
+        return new DafnyDocument(textDocument, errorReporter, program, symbolTable, serializedCounterExamples);
+      }
+
+      // Start binary search
+      while(begin < end){
+        int middle = (begin + end) / 2;
+        Console.WriteLine(">>>>>>>>>>>>>>>>>>>>>>>>>>> Current middle: " + middle + "<<<<<<<<<<<<<<<<<<<<<<<<");
+        errorReporter = new BuildErrorReporter();
+        program = await _parser.ParseAsync(textDocument, errorReporter, cancellationToken);
+        compilationUnit = await _symbolResolver.ResolveSymbolsAsync(textDocument, program, cancellationToken);
+        symbolTable = _symbolTableFactory.CreateFrom(program, compilationUnit, cancellationToken);
+        DocumentModifier.RemoveLemmaLines(program, "foo", "module1", middle);
+        serializedCounterExamples = await _verifier.VerifyAsync(program, cancellationToken);
+        if(errorReporter.AllMessages[ErrorLevel.Error].Count == 0){
+          begin = middle + 1;
+        }
+        else{
+          end = middle;
+        }
+      }
+      Console.WriteLine(">>>>>>>>>>>>>>>>>>>>>>>>>>> Final conclusion: assertion failure on line " + (begin - 1) + "<<<<<<<<<<<<<<<<<<<<<<<<");
+      int TargetLine = begin - 1;
+
+      // Perform the final pass, and record the lsp location of assertion failure
+      errorReporter = new BuildErrorReporter();
+      program = await _parser.ParseAsync(textDocument, errorReporter, cancellationToken);
+      compilationUnit = await _symbolResolver.ResolveSymbolsAsync(textDocument, program, cancellationToken);
+      symbolTable = _symbolTableFactory.CreateFrom(program, compilationUnit, cancellationToken);
+
+      foreach(ModuleDefinition module in program.ModuleSigs.Keys){
+          if(module.FullName != ModuleName) continue;
+          foreach(ICallable callable in module.CallGraph.vertices.Keys){
+              var corresVertex = module.CallGraph.vertices[callable];
+              if(callable.WhatKind != "lemma" || callable.NameRelativeToModule != LemmaName) continue;
+              var LemmaCallable = (Lemma)callable;
+              var Location = LemmaCallable.methodBody.Body[TargetLine].Tok.GetLspPosition();
+              var Range = LemmaCallable.methodBody.Body[TargetLine].Tok.GetLspRange();
+              Console.WriteLine(">>>>>>>>>>>>>>>>>>>>>>>>>>> " + Location);
+              Console.WriteLine(">>>>>>>>>>>>>>>>>>>>>>>>>>> " + Range.Start + " to " + Range.End);
+          }
+      }
+
+      serializedCounterExamples = await _verifier.VerifyAsync(program, cancellationToken);
+      _notificationPublisher.Completed(textDocument, serializedCounterExamples == null);
+      return new DafnyDocument(textDocument, errorReporter, program, symbolTable, serializedCounterExamples);
     }
   }
 }
