Source/DafnyLS.IntegrationTest/MyTest/TestFiles/ModuleTest.dfy
@@ -1,27 +1,10 @@
 module module1 {
-    method foo() {
-        assert 1 == 1;
-        assert true;
+    lemma foo() {
         assert false;
-    }
-
-    method bar() {
         assert 1 == 1;
         assert true;
-        foo();
-    }
-}
-
-module module2 {
-    method foo() {
-        assert 1 == 1;
+        assert 2 == 2;
         assert true;
-        assert false;
-    }
-
-    method bar() {
-        assert 1 == 1;
-        assert true;
-        foo();
+        assert 3 == 3;
     }
 }
